busy_beaver/impl.dfy
@@ -1,0 +1,27 @@
+include "defs.dfy"
+
+// Implementation of efficient methods mirroring specification in defs.dfy
+
+lemma StepNHalt(tm : TM, start_config : Config, n : nat, m : nat)
+  requires StepN(tm, start_config, n).state.Halt?
+  requires m >= n
+  ensures StepN(tm, start_config, m) == StepN(tm, start_config, n)
+
+method RunTM(tm : TM, start_config : Config, num_steps : nat) returns (end_config : Config)
+  ensures end_config == StepN(tm, start_config, num_steps)
+{
+  var i := 0;
+  var cur_config := start_config;
+  while i < num_steps && !cur_config.state.Halt?
+    invariant 0 <= i <= num_steps
+    invariant cur_config == StepN(tm, start_config, i)
+  {
+    cur_config := Step(tm, cur_config);
+    i := i + 1;
+  }
+  if cur_config.state.Halt? {
+    StepNHalt(tm, start_config, i, num_steps);
+  }
+  assert cur_config == StepN(tm, start_config, num_steps);
+  return cur_config;
+}
