busy_beaver/test_run.dfy
@@ -1,0 +1,13 @@
+include "defs.dfy"
+include "impl.dfy"
+include "parse.dfy"
+
+method RunTM(tm_str : string, num_steps : nat) {
+  var tm := ParseTM(tm_str);
+  var config := RunTM(tm, InitConfig, num_steps);
+  if config.state.Halt? {
+    print "TM Halted\n";
+  } else {
+    print "TM State: ", config.state.state, "\n";
+  }
+}
